Derived operations and theorems.

prototype/Is/Group.v
@@ -7,7 +7,12 @@ Import AdditiveNotations.
 Class IsGroup (A : Type) {has_eqv : HasEqv A}
   {has_opr : HasOpr A} {has_idn : HasIdn A} {has_inv : HasInv A} : Prop := {
   inv_proper : inv ::> eqv ==> eqv;
-  opr_idn_is_monoid :> IsMonoid A;
-  opr_idn_inv_is_left_inverse : IsLeftInverse A;
-  opr_idn_inv_is_right_inverse : IsRightInverse A;
+  opr_is_monoid :> IsMonoid A;
+  opr_is_left_inverse :> IsLeftInverse A;
+  opr_is_right_inverse :> IsRightInverse A;
 }.
+
+Add Parametric Morphism {A : Type} `{is_group : IsGroup A} : inv
+  with signature eqv ==> eqv
+  as eqv_inv_morphism.
+Proof. intros x y p. apply inv_proper; auto. Qed.
