prototype/Is/AbelianGroup.v
@@ -4,7 +4,7 @@ From Maniunfold.Is Require Import Group LeftIdentity RightIdentity.
 
 Class IsAbelianGroup (A : Type) {has_eqv : HasEqv A}
   {has_opr : HasOpr A} {has_idn : HasIdn A} {has_inv : HasInv A} : Prop := {
-  opr_idn_inv_is_group :> IsGroup A;
+  opr_is_group :> IsGroup A;
   opr_is_left_identity :> IsLeftIdentity A;
   opr_is_right_identity :> IsRightIdentity A;
 }.
