prototype/Is/CommutativeMonoid.v
@@ -3,6 +3,6 @@ From Maniunfold.Is Require Import Setoid Monoid Commutative.
 
 Class CommutativeMonoid (A : Type)
   {has_eqv : HasEqv A} {has_opr : HasOpr A} {has_idn : HasIdn A} : Prop := {
-  opr_idn_is_monoid :> IsMonoid A;
+  opr_is_monoid :> IsMonoid A;
   opr_commutative :> IsCommutative A;
 }.
