prototype/Shall/IntegerPower.v
@@ -1,0 +1,44 @@
+From Coq Require Import ZArith.
+From Maniunfold.Has Require Import Operation Identity Inverse.
+From Maniunfold.Is Require Import Semigroup Monoid Group.
+
+Import Pos.
+
+Definition popr {A : Type} `{is_semigroup : IsSemigroup A}
+  (n : positive) (x : A) : A :=
+  iter_op opr n x.
+
+Definition nopr {A : Type} `{is_monoid : IsMonoid A} (n : N) (x : A) : A :=
+  match n with
+  | N0 => idn
+  | Npos p => popr p x
+  end.
+
+Definition zopr {A : Type} `{is_group : IsGroup A} (n : Z) (x : A) : A :=
+  match n with
+  | Z0 => idn
+  | Zpos p => popr p x
+  | Zneg p => inv (popr p x)
+  end.
+
+Module AdditiveNotations.
+
+Export Inverse.AdditiveNotations.
+
+Reserved Notation "n '*^' x" (at level 40, left associativity).
+Notation "n '*^' x" := (popr n x) : positive_scope.
+Notation "n '*^' x" := (nopr n x) : N_scope.
+Notation "n '*^' x" := (zopr n x) : Z_scope.
+
+End AdditiveNotations.
+
+Module MultiplicativeNotations.
+
+Export Inverse.MultiplicativeNotations.
+
+Reserved Notation "x '*^' n" (at level 30, right associativity).
+Notation "x '*^' n" := (popr n x) : positive_scope.
+Notation "x '*^' n" := (nopr n x) : N_scope.
+Notation "x '*^' n" := (zopr n x) : Z_scope.
+
+End MultiplicativeNotations.
