prototype/Test.v
@@ -1,0 +1,107 @@
+From Coq Require Import ZArith.
+From Maniunfold.Has Require Import EquivalenceRelation
+  Operation Identity Inverse.
+From Maniunfold.Is Require Import Associative LeftIdentity RightIdentity
+  LeftInverse RightInverse Setoid Semigroup Monoid Group.
+From Maniunfold.Shall Require Import IntegerPower.
+
+Import AdditiveNotations Pos.
+
+Theorem inv_involutive : forall {A : Type} `{is_group : IsGroup A},
+  forall x : A, - (- x) == x.
+Proof.
+  intros A ? ? ? ? grp x.
+  rewrite <- (opr_right_identity (- (- x))). rewrite <- (opr_left_inverse x).
+  rewrite (opr_associative (- (- x)) (- x) x).
+  rewrite (opr_left_inverse (- x)). rewrite (opr_left_identity x).
+  reflexivity. Qed.
+
+Lemma opr_left_injective : forall {A : Type} `{is_group : IsGroup A},
+  forall x y z : A, z + x == z + y -> x == y.
+Proof.
+  intros A ? ? ? ? grp x y z p.
+  rewrite <- (opr_left_identity x). rewrite <- (opr_left_inverse z).
+  rewrite <- (opr_associative (- z) z x). rewrite p.
+  rewrite (opr_associative (- z) z y). rewrite (opr_left_inverse z).
+  rewrite (opr_left_identity y). reflexivity. Qed.
+
+Lemma opr_right_injective : forall {A : Type} `{is_group : IsGroup A},
+  forall x y z : A, x + z == y + z -> x == y.
+Proof.
+  intros A ? ? ? ? grp x y z p.
+  rewrite <- (opr_right_identity x). rewrite <- (opr_right_inverse z).
+  rewrite (opr_associative x z (- z)). rewrite p.
+  rewrite <- (opr_associative y z (- z)). rewrite (opr_right_inverse z).
+  rewrite (opr_right_identity y). reflexivity. Qed.
+
+Theorem opr_inv_distributive : forall {A : Type} `{is_group : IsGroup A},
+  forall x y : A, - (x + y) == (- y) + (- x).
+Proof.
+  intros A ? ? ? ? grp x y.
+  apply (opr_left_injective (- (x + y)) ((- y) + (- x)) (x + y)).
+  rewrite (opr_right_inverse (x + y)).
+  rewrite (opr_associative (x + y) (- y) (- x)).
+  rewrite <- (opr_associative x y (- y)). rewrite (opr_right_inverse y).
+  rewrite (opr_right_identity x). rewrite (opr_right_inverse x).
+  reflexivity. Qed.
+
+Theorem idn_inv_absorbing : forall {A : Type} `{is_group : IsGroup A},
+  - 0 == 0.
+Proof.
+  intros A ? ? ? ? grp.
+  rewrite <- (opr_right_identity (- 0)). rewrite (opr_left_inverse 0).
+  reflexivity. Qed.
+
+(** We need a setoid version of the standard library lemma [iter_op_succ]. *)
+Lemma iter_op_succ : forall {A : Type} `{is_setoid : IsSetoid A}
+  (op : A -> A -> A),
+  (forall x y z : A, op x (op y z) == op (op x y) z) ->
+  forall (n : positive) (x : A),
+  iter_op op (succ n) x == op x (iter_op op n x).
+Proof.
+  intros A ? ? op p n. induction n as [q r | q r |]; intros x.
+  - rewrite (p x x (iter_op op q (op x x))). rewrite (r (op x x)). reflexivity.
+  - reflexivity.
+  - reflexivity. Qed.
+
+Corollary iter_op_comm : forall {A : Type} `{is_setoid : IsSetoid A}
+  (op : A -> A -> A), (op ::> eqv ==> eqv ==> eqv) ->
+  (forall x y z : A, op x (op y z) == op (op x y) z) ->
+  forall (n : positive) (x : A),
+  op x (iter_op op n x) == op (iter_op op n x) x.
+Proof.
+  intros A ? ? op p q n x. induction n as [| r s] using peano_ind.
+  - reflexivity.
+  - rewrite (iter_op_succ op q r x). rewrite s.
+    rewrite (q x (iter_op op r x) x). rewrite <- s. reflexivity. Qed.
+
+Theorem popr_inv_distributive : forall {A : Type} `{is_group : IsGroup A},
+  forall (n : positive) (x : A),
+  (n *^ (- x) == - (n *^ x))%positive.
+Proof.
+  intros A ? ? ? ? grp n x. cbv [popr]. induction n as [| p q] using peano_ind.
+  - reflexivity.
+  - rewrite (iter_op_succ opr opr_associative p (- x)),
+      (iter_op_succ opr opr_associative p x).
+    rewrite q. rewrite <- (opr_inv_distributive (iter_op opr p x) x).
+    rewrite (iter_op_comm opr opr_proper opr_associative p x).
+    reflexivity. Qed.
+
+Theorem nopr_inv_distributive : forall {A : Type} `{is_group : IsGroup A},
+  forall (n : N) (x : A), (n *^ (- x) == - (n *^ x))%N.
+Proof.
+  intros A ? ? ? ? grp n x.
+  destruct n as [| p].
+  - cbv [nopr]. rewrite idn_inv_absorbing. reflexivity.
+  - cbv [nopr]. rewrite (popr_inv_distributive p x). reflexivity. Qed.
+
+Theorem zopr_inv_distributive : forall {A : Type} `{is_group : IsGroup A},
+  forall (n : Z) (x : A), (n *^ (- x)%inverse)%Z == - (n *^ x)%Z.
+Proof.
+  intros A ? ? ? ? grp n x.
+  destruct n as [| p | p].
+  - cbv [zopr]. rewrite idn_inv_absorbing. reflexivity.
+  - cbv [zopr]. rewrite (popr_inv_distributive p x). reflexivity.
+  - cbv [zopr]. rewrite (inv_involutive (p *^ x)%positive).
+    rewrite (popr_inv_distributive p x).
+    rewrite (inv_involutive (p *^ x)%positive). reflexivity. Qed.
